lawyer/nonblocking/examples/read_head.v
@@ -1,0 +1,291 @@
+From iris.base_logic Require Export gen_heap.
+From iris.proofmode Require Import tactics coq_tactics.
+From iris.bi.lib Require Import fixpoint.
+From trillium.program_logic Require Export weakestpre adequacy ectx_lifting.
+From fairness Require Import utils.
+From lawyer.examples Require Import obls_tactics.
+From lawyer.nonblocking.examples Require Import simple_queue_utils simple_queue.
+From lawyer.obligations Require Import obligations_model obligations_resources obligations_am obligations_em obligations_logic env_helpers.
+From lawyer Require Import sub_action_em program_logic.
+From iris.algebra Require Import auth gmap gset excl excl_auth csum mono_nat.
+From iris.base_logic.lib Require Import invariants.
+
+
+Close Scope Z.
+
+
+Section ReadHead.
+
+  Context {DegO LvlO LIM_STEPS} {OP: OP_HL DegO LvlO LIM_STEPS}.
+  Context `{EM: ExecutionModel heap_lang M}.
+  Notation "'Degree'" := (om_hl_Degree). 
+  Notation "'Level'" := (om_hl_Level).  
+
+  Context {Σ} {OHE: OM_HL_Env OP EM Σ}.
+  (* Existing Instance OHE.  *)
+  Context {QL: QueueG Σ}.
+
+  Context (d: Degree).
+
+  Let hGS: heap1GS Σ := iem_phys _ EM.
+  Existing Instance hGS.
+
+  Definition read_head_fuel := 100.
+
+  Definition get_head_val: val :=
+    λ: "ch1",
+      let: "ch2" := !#(Head q_sq) in
+      if: "ch1" = "ch2"
+      then get_val "ch1"
+      else !#(OldHeadVal q_sq)
+  .
+
+  (* TODO: move dequeue implementation to the corresponding file too *)
+  Definition read_head: val := 
+    λ: <>,
+       let: "ch" := !#(Head q_sq) in
+       let: "ct" := !#(Tail q_sq) in
+       if: "ch" = "ct" then NONE
+       else
+         #(BeingRead q_sq) <- "ch" ;;
+         SOME (get_head_val "ch")
+  .
+
+  (* TODO: move *)
+  Lemma read_head_resources_excl t1 br1 pt1 rop1 t2 br2 pt2 rop2:
+    read_head_resources t1 br1 pt1 rop1 -∗ read_head_resources t2 br2 pt2 rop2 -∗ False.
+  Proof using.
+    simpl. rewrite /read_head_resources.
+    iIntros "(X&_) (Y&_)".
+    by iApply (me_exact_excl with "X [$]"). 
+  Qed.
+
+  Lemma read_head_resources_auth_agree t' br' pt' rop' h t br fl:
+    read_head_resources t' br' pt' rop' -∗ auths h t br fl -∗ ⌜ t' = t /\ br' = br ⌝.
+  Proof using.
+    simpl. iIntros "(T&BR&_) (?&T'&BR'&_)".
+    iDestruct (me_auth_exact with "T' T") as %?. 
+    iDestruct (me_auth_exact with "BR' BR") as %?.
+    done. 
+  Qed. 
+    
+  Lemma read_head_resources_rop_interp_agree t' br' pt' rop' hist rop h br fl od:
+    read_head_resources t' br' pt' rop' -∗ read_hist_interp hist rop h br fl od -∗
+    ⌜ rop' = rop ⌝.
+  Proof using.
+    simpl. rewrite /read_hist_interp.  
+    iIntros "(T&BR&?&ROP) (ROP'&_)".
+    iCombine "ROP' ROP" as "R". 
+    iDestruct (own_valid with "R") as %V.
+    iPureIntro. symmetry. by apply excl_auth_agree_L.
+  Qed.
+    
+  Lemma read_head_token_excl:
+    read_head_token -∗ read_head_token -∗ False.
+  Proof using.
+    simpl. 
+    rewrite bi.wand_curry -own_op.
+    iIntros "X". by iDestruct (own_valid with "[$]") as %V.
+  Qed. 
+
+  (* TODO: move, remove duplicates *)
+  Lemma dom_max_set_fold n:
+    set_fold max 0 (set_seq 0 (S n): gset nat) = n.
+  Proof using.
+    clear. induction n.
+    { done. }
+    rewrite set_seq_S_end_union_L.
+    rewrite union_comm_L. 
+    erewrite set_fold_union.
+    2-4: red; lia.
+    simpl. rewrite IHn.
+    rewrite set_fold_singleton. lia.
+  Qed.
+
+  Lemma read_hist_alloc (hist: read_hist) h
+    (RH_WF: read_hist_wf hist None h)
+    (n' := set_fold max 0 (dom hist) + 1):
+    read_hist_auth hist ==∗
+    let hist' := <[ n' := ((h, h), rs_init) ]> hist in
+    read_hist_auth hist' ∗ ith_read n' h h ∗ ⌜ read_hist_wf hist' (Some n') h ⌝ ∗
+    ith_rp n' rs_init.
+  Proof using.
+    simpl. iIntros "AUTH".
+    destruct RH_WF as (n & DOM & ROP & SEQ & BB).
+    clear ROP.
+
+    assert (n' = S n) as ->.
+    { subst n'. rewrite DOM dom_max_set_fold. lia. }    
+    
+    iMod (read_hist_alloc hist (S n) h h rs_init with "AUTH") as "(AUTH & #ITH & RP)".
+    { rewrite DOM. rewrite elem_of_set_seq. lia. }
+    iFrame "#∗". 
+    iPureIntro. red. 
+        
+    exists (S n). split; [| split; [| split]]. 
+    - rewrite dom_insert_L. rewrite DOM.
+      rewrite !set_seq_S_end_union_L. set_solver. 
+    - tauto.
+    - intros ?????. rewrite !lookup_insert_Some.
+      intros [(? & ?) | (? & ITH) ] [(? & ?) | (? & JTH) ]; subst; simpl in *; try lia.
+      + apply mk_is_Some, elem_of_dom in JTH.
+        rewrite DOM elem_of_union elem_of_set_seq elem_of_singleton in JTH. lia.
+      + eapply BB; eauto. 
+      + eapply SEQ in H; eauto; try done.
+    - intros ??. rewrite lookup_insert_Some.         
+      intros [(? & ?) | (? & ITH) ]; subst; simpl; try lia.
+      eapply BB in ITH; eauto. 
+  Qed.
+    
+  Lemma rop_update rop1 rop2 rop':
+    rop_auth rop1 -∗ rop_frag rop2 ==∗ rop_auth rop' ∗ rop_frag rop'. 
+  Proof using.
+    simpl. rewrite /rop_auth /rop_frag.
+    rewrite bi.wand_curry -!own_op.
+    iApply own_update. apply excl_auth_update. 
+  Qed.  
+
+  Lemma start_rop hist rop_ h br pt fl od t:
+  read_hist_interp hist rop_ h br fl od -∗ read_head_resources t br pt None ==∗
+  ∃ i hist', read_hist_interp hist' (Some i) h br fl od ∗ read_head_resources t br pt (Some i) ∗ 
+              ith_read i h h.
+  Proof using.
+    iIntros "ROP RH".
+    iDestruct (read_head_resources_rop_interp_agree with "[$] [$]") as %<-.
+    rewrite {1}/read_hist_interp {1}/read_head_resources.
+    iDestruct "ROP" as "(ROPA & ROP & RHIST & %RH_WF & #OLDS)".
+    iDestruct "RH" as "(TLA & BRA & TAIL & ROPF)".
+    rewrite /rop_interp. iClear "ROP".
+
+    iMod (read_hist_alloc with "[$]") as "(AUTH & #READ & %RH_WF' & RP)"; [done| ].
+    red in RH_WF.
+    destruct RH_WF as (n & DOM & ROP & SEQ & BB).
+    assert (set_fold Init.Nat.max 0 (dom hist) + 1 = S n) as EQ. 
+    { rewrite DOM dom_max_set_fold. lia. }
+    rewrite EQ. rewrite EQ in RH_WF'.
+
+    iMod (rop_update _ _ (Some (S n)) with "[$] [$]") as "(ROPA & ROPF)". 
+    iFrame "#∗".
+    iModIntro. iSplitL.
+    2: { iSplit; [done| ].
+         iApply old_rps_olds. rewrite delete_insert; [done| ].
+         apply not_elem_of_dom. rewrite DOM. rewrite elem_of_set_seq. lia. }
+    rewrite /rop_interp. iIntros (? [=<-]).
+    iFrame "RP". iExists _. iSplit.
+    { iApply (ith_included with "READ"). lia. }
+    iLeft. rewrite /safe_read. iLeft. iSplit; try done.
+    by iLeft.
+  Qed.
+
+  Definition h_lb (b: nat) := @me_lb _ q_me_h b.
+
+  Lemma h_lb_bound b h t br fl:
+    h_lb b -∗ auths h t br fl -∗ ⌜ b <= h ⌝.
+  Proof using.
+    iIntros "LB (H&?&?&?)".
+    iApply (me_auth_lb with "H LB").
+  Qed.  
+
+  Lemma read_head_res_Tail_agree t br pt rop pt':
+    read_head_resources t br pt rop -∗ Tail q_sq ↦{1 / 2} #pt' -∗ ⌜ pt' = pt ⌝.
+  Proof using.
+    simpl. rewrite /read_head_resources. iIntros "(_&_&T&?) T'".
+    iDestruct (pointsto_agree with "[$] [$]") as %?. set_solver.
+  Qed.
+    
+  Lemma read_head_spec l (τ: locale heap_lang) (π: Phase) (q: Qp):
+    {{{ queue_inv l ∗ read_head_token ∗ 
+        th_phase_frag τ π q ∗ cp_mul π d read_head_fuel }}}
+       read_head #() @ τ
+    {{{ (v: val), RET v; th_phase_frag τ π q ∗ read_head_token }}}.
+  Proof using.
+    simpl. iIntros (Φ) "([#QAT #INV] & TOK & PH & CPS) POST".
+    rewrite /read_head. destruct q_sq eqn:Q_SQ.
+    pure_steps.
+
+    wp_bind (! _)%E.
+    iInv "INV" as "(%hq & %h0 & %t & %br & %fl0 & %rop & %od & %hist & inv)" "CLOS".
+    iEval (rewrite /queue_inv_inner) in "inv".
+    iDestruct "inv" as ">(HQ & AUTHS & %ORDER0 & QI & DANGLE & OHV & RHI & RH & DQ)".
+    
+    iApply sswp_MU_wp; [done| ].
+    iDestruct (access_queue_ends with "[$] [$]") as "(%ph & %pt & HEAD & TAIL & #HT & CLOS')".
+    replace Head with (simple_queue.Head q_sq) by (by rewrite Q_SQ).
+    iApply (wp_load with "HEAD"). iIntros "!> HEAD".
+    iDestruct "RH" as "[(%pt_ & RH) | TOK']".
+    2: { by iDestruct (read_head_token_excl with "[$] [$]") as "?". }
+    iDestruct (read_head_res_Tail_agree with "RH [$]") as %EQ.
+    inversion EQ. subst pt_. clear EQ. 
+    iAssert (h_lb h0)%I as "#H_LB". 
+    { iDestruct (take_snapshot with "[$]") as "($&?&?&?)". }
+      
+    iDestruct ("CLOS'" with "[$] [$]") as "(HQ & QI)".
+    MU_by_burn_cp. iApply wp_value.
+
+    iMod (start_rop with "RHI RH") as "(%i & %hist' & RHI & RH & #ITH)". 
+
+    iMod ("CLOS" with "[-POST CPS PH RH]") as "_".
+    { by iFrame. }
+    iModIntro. clear hist hq od fl0 ORDER0 rop hist'. 
+
+    wp_bind (Rec _ _ _)%E. pure_steps.
+    wp_bind (! _)%E.
+    iInv "INV" as "(%hq & %h1 & %t_ & %br_ & %fl1 & %rop_ & %od & %hist & inv)" "CLOS".
+    iEval (rewrite /queue_inv_inner) in "inv".
+    iDestruct "inv" as ">(HQ & AUTHS & %ORDER1 & QI & DANGLE & OHV & RHI & RH' & DQ)".
+    (* iDestruct (h_lb_bound with "[$] [$]") as %H01.  *)
+    iApply sswp_MU_wp; [done| ].
+    iDestruct (access_queue_ends with "[$] [$]") as "(%ph' & %pt_ & HEAD & TAIL & _ & CLOS')".
+    iDestruct (read_head_res_Tail_agree with "RH [$]") as %EQ.
+    inversion EQ. subst pt_. clear EQ.
+    replace Tail with (simple_queue.Tail q_sq) by (by rewrite Q_SQ).
+    iApply (wp_load with "TAIL"). iIntros "!> TAIL".
+    iDestruct "RH'" as "[(% & RH') | TOK]".
+    { by iDestruct (read_head_resources_excl with "RH RH'") as "?". }
+    iDestruct ("CLOS'" with "[$] [$]") as "(HQ & QI)".
+    MU_by_burn_cp. iApply wp_value.
+    iMod ("CLOS" with "[-POST CPS PH RH]") as "_".
+    { by iFrame. }
+    iModIntro. clear hist hq rop_ ph' od br_ ORDER1 h1 t_ fl1.
+
+    wp_bind (Rec _ _ _)%E. pure_steps.
+
+    wp_bind (_ = _)%E.
+    iApply sswp_MU_wp; [done| ].
+    iApply sswp_pure_step.
+    { set_solver. }
+    MU_by_burn_cp. iApply wp_value.
+
+    iDestruct "HT" as "[[%EMPTY ->] | ([%NEMPTY %NEQ] & (%ndh0 & #HTH0))]".
+    { rewrite bool_decide_true; [| done].
+
+      iApply sswp_MU_wp_fupd; [done| ].
+      iClear "H_LB ITH". clear dependent h0.
+
+      iInv "INV" as "(%hq & %h1 & %t_ & %br_ & %fl1 & %rop_ & %od & %hist & inv)" "CLOS".
+      iEval (rewrite /queue_inv_inner) in "inv".
+      iDestruct "inv" as ">(HQ & AUTHS & %ORDER1 & QI & DANGLE & OHV & RHI & RH' & DQ)".
+      iModIntro. 
+ 
+      iApply sswp_pure_step.
+      { set_solver. }
+      MU_by_burn_cp.
+      iDestruct "RH'" as "[(% & RH') | TOK]".
+      { by iDestruct (read_head_resources_excl with "RH RH'") as "?". }
+      iMod ("CLOS" with "[-POST CPS PH TOK]") as "_".
+      { iDestruct (read_head_resources_rop_interp_agree with "[$] [$]") as %<-. 
+        iDestruct (read_head_resources_auth_agree with "[$] [$]") as %[<- <-]. 
+        iFrame. iNext. iSplit; [done| ].
+        by iLeft. 
+      }
+
+
+      
+      
+      pure_steps. iApply "POST". iFrame. }
+
+    rewrite PTR_EQ. 
+
+  
+
+End ReadHead. 
